clean up

Library/Random.dfy
@@ -27,99 +27,41 @@ module {:extern "DafnyLibraries"} DafnyLibraries {
       modifies this
       ensures Model.Coin(old(s)) == (b, s)
 
-/*     // Based on https://arxiv.org/pdf/1304.1916.pdf; unverified.
-    method Uniform(n: nat) returns (m: nat)
-      requires n > 0
-      ensures Model.Uniform(n)(old(s)) == (m, s)
+    // Based on https://arxiv.org/pdf/1304.1916.pdf; unverified.
+    method Uniform(n: nat) returns (u: nat)
+      modifies this
+      requires 0 < n
+      ensures Model.Uniform(n)(old(s)) == (u, s)
+      decreases *
     {
       assume {:axiom} false;
       var v := 1;
-      m := 0;
+      u := 0;
       while true {
         v := 2 * v;
         var b := Coin();
-        m := if b then 2*m + 1 else 2*m;
+        u := 2 * u + if b then 1 else 0;
         if v >= n {
-          if m < n {
+          if u < n {
             return;
           } else {
             v := v - n;
-            m := m - n;
+            u := u - n;
           }
-        }
-      } */
-/*       while true
-        decreases *
-      {
-        var (m, s) := ProbUnif(n-1)(s);
-        if m < n {
-          return (m, s);
-        }
-      } 
-    }*/
-
- /*    method Unif2(n: nat) returns (m: nat) 
-      decreases *
-      ensures Unif.ProbUnif(n)(old(s)) == (m, s)
-    {
-      m := 0;
-
-      if n == 0 {
-        return m;
-      } else {
-        var b := Coin();
-        m := if b then 2*m + 1 else 2*m;
-        var n := n / 2;
-      }
-
-      while true
-        decreases *
-        invariant m >= 0 && (n == 0 ==> Unif.ProbUnif(n)(old(s)) == (m, s))
-      {
-        if n == 0 {
-          return m;
-        } else {
-          var b := Coin();
-          m := if b then 2*m + 1 else 2*m;
-          var n := n / 2;
-        }
-      }
-    } */
-
-    method {:timeLimit 20} Uniform(n: nat) returns (m: nat)
-      modifies this
-      requires n > 0
-      ensures Model.Uniform(n)(old(s)) == (m, s)
-      decreases *
-    {
-      assume {:axiom} false;
-      m := 0;
-      var n := n - 1;
-
-      while true 
-        decreases *
-        invariant m >= 0 && (n == 0 && m < n ==> Model.Uniform(n)(old(s)) == (m, s))
-      {
-        if n != 0 {
-          var b := Coin();
-          m := if b then 2*m + 1 else 2*m;
-          var n := n / 2;
-        } else if m < n {
-          return m;
         }
       }
     }
-
-    method UniformInterval(a: int, b: int) returns (m: int)
+    
+    method UniformInterval(a: int, b: int) returns (u: int)
       modifies this
       requires a < b
-      ensures Model.UniformInterval(a, b)(old(s)) == (m, s)
+      ensures Model.UniformInterval(a, b)(old(s)) == (u, s)
       decreases *
     {
       var v := Uniform(b - a);
       assert Model.Uniform(b-a)(old(s)) == (v, s);
       assert Model.UniformInterval(a, b)(old(s)) == (a + v, s);
-      m := a + v;
+      u := a + v;
     }
 
     method Bernoulli(p: real) returns (c: bool)
